Logic/Modal/Normal/Formula.lean
@@ -30,6 +30,12 @@ instance : ModalLogicSymbol (Formula α) where
   box := box
   dia := dia
 
+instance : NegDefinition (Formula α) where
+  neg := rfl
+
+instance : ModalDuality (Formula α) where
+  dia := rfl
+
 section ToString
 
 variable [ToString α]
@@ -60,13 +66,13 @@ lemma iff_eq (p q : Formula α) : p ⟷ q = (p ⟶ q) ⋏ (q ⟶ p) := rfl
 
 lemma dia_eq (p : Formula α) : ◇p = ~(□(~p)) := rfl
 
-@[simp] lemma neg_inj (p q : Formula α) : ~p = ~q ↔ p = q := by simp[neg_eq, neg, *]
-
 @[simp] lemma and_inj (p₁ q₁ p₂ q₂ : Formula α) : p₁ ⋏ p₂ = q₁ ⋏ q₂ ↔ p₁ = q₁ ∧ p₂ = q₂ := by simp[Wedge.wedge]
 
 @[simp] lemma or_inj (p₁ q₁ p₂ q₂ : Formula α) : p₁ ⋎ p₂ = q₁ ⋎ q₂ ↔ p₁ = q₁ ∧ p₂ = q₂ := by simp[Vee.vee]
 
 @[simp] lemma imp_inj (p₁ q₁ p₂ q₂ : Formula α) : p₁ ⟶ p₂ = q₁ ⟶ q₂ ↔ p₁ = q₁ ∧ p₂ = q₂ := by simp[Arrow.arrow]
+
+@[simp] lemma neg_inj (p q : Formula α) : ~p = ~q ↔ p = q := by simp[*]
 
 @[simp] lemma box_inj (p q : Formula α) : □p = □q ↔ p = q := by simp[Box.box]
 
